Adjust single-step semantics to make relabelling easier.
New rule says

  (m0, IfStmt gd th el) --> (m0, Seq [Done; c])

where c is one of th or el, depending on how the guard evaluates.
The bogus insertion of a Done command (a Skip if you will) ensures
that when you create a nested graph on the left and a graph on the
right, you will end up with the same number of nodes.

On the left, you get a readAction corresponding to the expression
evaluation and one for the command. On the right you will get one for
the Done, and one for the command. The fact that the node on the right
for the Done will just contain an empty graph is neither here nor
there.

hol/PseudoCPropsScript.sml
@@ -33,11 +33,10 @@ val stmt_weight_def = tDefine "stmt_weight" `
      1 + ew (SND w) + SUM (MAP dw ds)) ∧
   (stmt_weight (AssignVar v ds vf) = 1 + SUM (MAP dw ds)) ∧
   (stmt_weight (Malloc v d value) = 1) ∧
-  (stmt_weight (IfStmt g t e) = MAX (stmt_weight t) (stmt_weight e) + 1) ∧
+  (stmt_weight (IfStmt g t e) = MAX (stmt_weight t) (stmt_weight e) + 3) ∧
   (stmt_weight (ForLoop v d s) = stmt_weight s + 1) ∧
   (stmt_weight (ParLoop v d s) = stmt_weight s + 1) ∧
-  (stmt_weight (Seq stmts) =
-    SUM (MAP stmt_weight stmts) + 1 + LENGTH stmts) ∧
+  (stmt_weight (Seq stmts) = SUM (MAP stmt_weight stmts) + LENGTH stmts) ∧
   (stmt_weight (Par stmts) =
     SUM (MAP stmt_weight stmts) + 1 + LENGTH stmts)
 ` (WF_REL_TAC `measure stmt_size` >> simp[] >>
@@ -45,19 +44,34 @@ val stmt_weight_def = tDefine "stmt_weight" `
    rpt strip_tac >> res_tac >> simp[])
 val _ = export_rewrites ["stmt_weight_def"]
 
+
+val seq_count_def = tDefine "seq_count" `
+  (seq_count (Seq cs) = SUM (MAP seq_count cs) + 1) ∧
+  (seq_count (Par cs) = SUM (MAP seq_count cs) + 1) ∧
+  (seq_count (ParLoop v d s) = seq_count s) ∧
+  (seq_count (ForLoop v d s) = seq_count s) ∧
+  (seq_count (IfStmt g t e) = seq_count t + seq_count e) ∧
+  (seq_count _ = 0)
+`
+  (WF_REL_TAC `measure stmt_size` >> simp[] >> Induct >> simp[] >>
+   rpt strip_tac >> simp[stmt_size_def] >> res_tac >> simp[])
+val _ = export_rewrites ["seq_count_def"]
+
 val loopbag_def = tDefine "loopbag" `
-  (loopbag Abort = {| 0 |}) ∧
-  (loopbag Done = {| 0 |}) ∧
-  (loopbag (Assign w ds v) = {| 0 |}) ∧
-  (loopbag (AssignVar v ds vf) = {| 0 |}) ∧
-  (loopbag (Malloc v d value) = {| 0 |}) ∧
+  (loopbag Abort = {| |}) ∧
+  (loopbag Done = {| |}) ∧
+  (loopbag (Assign w ds v) = {| |}) ∧
+  (loopbag (AssignVar v ds vf) = {| |}) ∧
+  (loopbag (Malloc v d value) = {| |}) ∧
   (loopbag (IfStmt g t e) = BAG_UNION (loopbag t) (loopbag e)) ∧
-  (loopbag (ForLoop v d s) = BAG_IMAGE SUC (loopbag s)) ∧
-  (loopbag (ParLoop v d s) = BAG_IMAGE SUC (loopbag s)) ∧
+  (loopbag (ForLoop v d s) = if loopbag s = {||} then {|1|}
+                             else BAG_IMAGE SUC (loopbag s)) ∧
+  (loopbag (ParLoop v d s) = if loopbag s = {||} then {|1|}
+                             else BAG_IMAGE SUC (loopbag s)) ∧
   (loopbag (Seq stmts) =
-     FOLDR (λms b. BAG_UNION (loopbag ms) b) {|0|} stmts) ∧
+     FOLDR (λms b. BAG_UNION (loopbag ms) b) {||} stmts) ∧
   (loopbag (Par stmts) =
-     FOLDR (λms b. BAG_UNION (loopbag ms) b) {|0|} stmts)
+     FOLDR (λms b. BAG_UNION (loopbag ms) b) {||} stmts)
 ` (WF_REL_TAC `measure stmt_size` >> simp[] >>
    Induct >> dsimp[stmt_size_def] >>
    rpt strip_tac >> res_tac >> simp[])
@@ -67,13 +81,8 @@ val FINITE_loopbag = store_thm(
   "FINITE_loopbag[simp]",
   ``∀s. FINITE_BAG (loopbag s)``,
   ho_match_mp_tac (theorem "loopbag_ind") >>
-  simp[] >> Induct >> simp[]);
-
-val loopbag_not_empty = store_thm(
-  "loopbag_not_empty[simp]",
-  ``∀s. loopbag s ≠ {||}``,
-  ho_match_mp_tac (theorem "loopbag_ind") >> simp[] >>
-  Induct >> simp[]);
+  simp[] >> reverse (rpt conj_tac)
+  >- (Induct >> simp[]) >> rw[]);
 
 val MAX_PLUS = store_thm(
   "MAX_PLUS",
@@ -115,16 +124,19 @@ val FINITE_BAG_FOLDR_loopbag = store_thm(
 
 val mlt_loopbag_lemma = store_thm(
   "mlt_loopbag_lemma",
-  ``mlt $< (FOLDR (λx b. BAG_UNION (loopbag s) b) {|0|} list)
+  ``loopbag s ≠ {||} ⇒
+    mlt $< (FOLDR (λx b. BAG_UNION (loopbag s) b) {||} list)
            (BAG_IMAGE SUC (loopbag s))``,
-  simp[mlt_dominates_thm1] >> qexists_tac `BAG_IMAGE SUC (loopbag s)` >>
+  simp[mlt_dominates_thm1] >> strip_tac >>
+  qexists_tac `BAG_IMAGE SUC (loopbag s)` >>
   simp[] >> dsimp[dominates_def] >>
   qho_match_abbrev_tac
     `∀e1. BAG_IN e1 FF ⇒ ∃e2. BAG_IN e2 (loopbag s) /\ e1 < SUC e2` >>
-  `∀e. BAG_IN e FF ⇒ BAG_IN e (loopbag s) ∨ e = 0`
-    by (simp[Abbr`FF`] >> Induct_on `list` >> simp[] >> metis_tac[]) >>
-  rpt strip_tac >> res_tac >- metis_tac[DECIDE ``x < SUC x``] >> simp[] >>
-  metis_tac[loopbag_not_empty, BAG_cases, BAG_IN_BAG_INSERT]);
+  `list ≠ [] ⇒ ∀e. BAG_IN e FF ⇒ BAG_IN e (loopbag s)`
+    by (simp[Abbr`FF`] >> Induct_on `list` >> simp[] >>
+        Cases_on `list` >> fs[] >> metis_tac[]) >>
+  rpt strip_tac >> Cases_on `list` >> fs[] >- fs[Abbr`FF`] >>
+  res_tac >> metis_tac[DECIDE ``x < SUC x``])
 
 val FORALL_domain = store_thm(
   "FORALL_domain",
@@ -139,11 +151,14 @@ val loopbag_ssubst = store_thm(
     [ssubst_def, FORALL_domain] >>
   simp[FOLDR_MAP,
       Cong (SPEC_ALL
-              (REWRITE_RULE [GSYM AND_IMP_INTRO] FOLDR_CONG))]);
+              (REWRITE_RULE [GSYM AND_IMP_INTRO] FOLDR_CONG))] >>
+  metis_tac[]);
 
 val _ = overload_on (
   "evalR",
-  ``inv_image (mlt (<) LEX (<)) (λ(m:memory,s). (loopbag s, stmt_weight dexpr_weight expr_weight s))``
+  ``inv_image (mlt (<) LEX (<) LEX (<))
+      (λ(m:memory,s). (loopbag s, stmt_weight dexpr_weight expr_weight s,
+                       seq_count s))``
 )
 
 val WF_evalR = store_thm(
@@ -160,6 +175,36 @@ val WF_eval_induction =
       |> SIMP_RULE (srw_ss()) []
       |> Q.GEN `Q`
 
+val mlt_FINITE_BAG = store_thm(
+  "mlt_FINITE_BAG",
+  ``∀s1 s2. mlt R s1 s2 ⇒ FINITE_BAG s1 ∧ FINITE_BAG s2``,
+  Induct_on `TC` >> simp[mlt1_def]);
+
+val mlt_EMPTY_BAG = store_thm(
+  "mlt_EMPTY_BAG[simp]",
+  ``mlt R {||} s ⇔ FINITE_BAG s ∧ s ≠ {||}``,
+  eq_tac
+  >- (`∀s1 s2. mlt R s1 s2 ⇒ s1 = {||} ⇒ FINITE_BAG s2 ∧ s2 ≠ {||}`
+        suffices_by metis_tac[] >>
+      Induct_on `TC` >> simp[] >> rpt strip_tac >>
+      fs[mlt1_def] >> imp_res_tac mlt_FINITE_BAG) >>
+  `∀s. FINITE_BAG s ⇒ s ≠ {||} ⇒ mlt R {||} s`
+    suffices_by metis_tac[] >>
+  Induct_on `FINITE_BAG` >> simp[] >> qx_gen_tac `b` >>
+  strip_tac >> qx_gen_tac `e` >> Cases_on `b = {||}` >> fs[]
+  >- (match_mp_tac relationTheory.TC_SUBSET >> simp[mlt1_def]) >>
+  `mlt R b (BAG_INSERT e b)`
+    by (match_mp_tac relationTheory.TC_SUBSET >>
+        simp[mlt1_def] >> map_every qexists_tac [`e`, `{||}`, `b`] >>
+        simp[] >> simp[BAG_EXTENSION, BAG_INN, BAG_INSERT, BAG_UNION,
+                       EMPTY_BAG] >>
+        map_every qx_gen_tac [`m`, `d`] >> Cases_on `d = e` >> simp[]) >>
+  metis_tac[relationTheory.TC_RULES]);
+
+val FOLDR_KI = store_thm(
+  "FOLDR_KI[simp]",
+  ``FOLDR (\e a. a) acc list = acc``,
+  Induct_on `list` >> simp[]);
 
 val eval_terminates = store_thm(
   "eval_terminates",
@@ -168,25 +213,23 @@ val eval_terminates = store_thm(
   lfs[LEX_DEF, MAX_SET_THM, SUM_APPEND]
   >- (Induct_on `pfx` >> simp[])
   >- (Induct_on `pfx` >> simp[])
-  >- (simp[mltLT_SING0] >> Induct_on `cs` >> simp[] >>
-      metis_tac[BAG_UNION_LEFT_CANCEL, BAG_UNION_EMPTY])
-  >- (Cases_on `b` >> simp[])
-  >- (simp[mltLT_SING0] >> metis_tac[])
+  >- (Induct_on `pfx` >> simp[])
+  >- (metis_tac[])
+  >- (Cases_on `b` >> simp[MAX_PLUS])
+  >- (metis_tac[])
   >- (Cases_on `e` >> fs[isValue_def])
   >- (Cases_on `expr` >> fs[isValue_def])
   >- (Cases_on `expr` >> fs[isValue_def])
-  >- simp[FOLDR_MAP, mlt_loopbag_lemma]
-  >- (simp[mltLT_SING0] >> metis_tac[])
-  >- (simp[FOLDR_MAP, mlt_loopbag_lemma])
-  >- (simp[mltLT_SING0] >> metis_tac[])
+  >- (rw[] >> simp[FOLDR_MAP, mlt_loopbag_lemma])
+  >- (rw[])
+  >- (rw[] >> simp[FOLDR_MAP, mlt_loopbag_lemma])
+  >- (rw[])
   >- (disj1_tac >> rw[] >> Induct_on `pfx` >> simp[] >>
       Induct_on `sfx` >> simp[])
-  >- (disj2_tac >> simp[SUM_APPEND] >> rw[] >>
-      Induct_on `pfx` >> simp[])
-  >- (simp[mltLT_SING0] >> Induct_on `cs` >> simp[] >>
-      metis_tac[BAG_UNION_LEFT_CANCEL, BAG_UNION_EMPTY])
-  >- (simp[mltLT_SING0] >> Induct_on `cs` >> simp[] >>
-      rw[] >> simp[] >> metis_tac[BAG_UNION_LEFT_CANCEL, BAG_UNION_EMPTY]));
+  >- (disj2_tac >> rw[] >> Induct_on `pfx` >> simp[])
+  >- (disj2_tac >> rw[] >> Induct_on `pfx` >> simp[])
+  >- (metis_tac[])
+  >- (metis_tac[]));
 
 (* ----------------------------------------------------------------------
     Create an action graph from a PseudoC program.
@@ -210,8 +253,8 @@ val OPT_SEQUENCE_def = Define`
 val MEM_FOLDR_mlt = store_thm(
   "MEM_FOLDR_mlt",
   ``MEM e l ⇒
-    mlt $< (loopbag (f e)) (FOLDR (\e a. loopbag (f e) ⊎ a) {|0|} l) ∨
-    loopbag (f e) = FOLDR (\e a. loopbag (f e) ⊎ a) {|0|} l``,
+    mlt $< (loopbag (f e)) (FOLDR (\e a. loopbag (f e) ⊎ a) {||} l) ∨
+    loopbag (f e) = FOLDR (\e a. loopbag (f e) ⊎ a) {||} l``,
   Induct_on `l` >> dsimp[] >> rpt strip_tac >> res_tac
   >- (Cases_on `loopbag (f h) = {||}` >> simp[] >>
       disj1_tac >>
@@ -844,7 +887,7 @@ val graphOf_def = tDefine "graphOf" `
 ` (WF_REL_TAC
      `inv_image (mlt (<) LEX (<)) (λ(i,m,s). (loopbag s, stmt_weight (K 0) (K 0) s))` >>
    simp[WF_mlt1, FOLDR_MAP, mlt_loopbag_lemma] >>
-   rpt strip_tac
+   rpt strip_tac >> TRY (rw[mlt_loopbag_lemma, MAX_PLUS] >> NO_TAC)
    >- (imp_res_tac MEM_FOLDR_mlt >> pop_assum (qspec_then `I` mp_tac) >>
        rw[] >> simp[] >> qpat_assum `MEM c cmds` mp_tac >>
        rpt (pop_assum kall_tac) >>
@@ -2330,6 +2373,7 @@ val graphOf_correct_lemma = store_thm(
   >- ((* guard of if evaluates to boolean and next statement selected *)
       map_every qx_gen_tac [`m0`, `gd`, `t`, `e`, `b`] >>
       rpt gen_tac >> strip_tac >> simp[Once graphOf_def, SimpL ``$==>``] >>
+      simp[graphOf_def, SimpR ``$==>``] >>
       Cases_on `b` >> simp[EXISTS_PROD, PULL_EXISTS, FORALL_PROD] >>
       map_every qx_gen_tac [`i0`, `i`, `m`, `g`] >>
       strip_tac >>
